save

sf/imp.lean
@@ -1,164 +1,511 @@
-
--- Inspired by Software Foundations Vol. 1: Imp chapter
+-- Some simple programming language modeling, using lean4
+-- commit 4296e1d83e734b18b4787329e4195569c0518325 
+-- from Fri Mar 20 18:32:04 2020 -0700
+import Init.Data.String
 
 -- -- -- -- -- -- -- -- -- -- -- -- -- -- -- -- --
 -- Data definitions
 -- -- -- -- -- -- -- -- -- -- -- -- -- -- -- -- --
 
+def Var := String
+
 -- Arithmetic unary operations
-inductive AUOp
-| inc : AUOp
-| dec : AUOp
+inductive Ty : Type
+| int : Ty
+| bool : Ty
+--|sum : Ty → Ty → Ty
 
 -- Arithmetic binary operations
-inductive ABOp
-| add : ABOp
-| sub : ABOp
-| mul : ABOp
+inductive Const : Type
+| int : Int → Const
+| bool : Bool → Const
+--|left : Const → Ty → Const
+--|right : Ty → Const → Const
+
+instance intToConst : HasCoe Int Const := ⟨Const.int⟩
+instance boolToConst : HasCoe Bool Const := ⟨Const.bool⟩
+
+inductive UOp : Type
+| inc
+| dec
+| neg
+| zero?
+| not
+
+inductive BOp : Type
+| add
+| sub
+| mul
+  
 
 -- Arithmetic expressions
-inductive AExp
-| num : Nat → AExp
-| var : String → AExp
-| uop : AUOp → AExp → AExp
-| bop : ABOp → AExp → AExp → AExp
+inductive Exp : Type
+| var    : Var → Exp
+| const  : Const → Exp
+| uop    : UOp → Exp → Exp
+| bop    : BOp → Exp → Exp → Exp
+| cond   : Exp → Exp → Exp → Exp
+| letvar : Var → Exp → Exp → Exp
+--|left  : Exp → Ty → Exp
+--|right : Ty → Exp → Exp
+--|elim  : Exp → Ty → Ty → Var
 
--- Boolean-returning arithmetic binary operations
-inductive BBOp
-| eq  : BBOp
-| le  : BBOp
 
--- Boolean expressions
-inductive BExp
-| bool : Bool → BExp
-| bop  : BBOp → AExp → AExp → BExp
-| not  : BExp → BExp
-| and  : BExp → BExp → BExp
-| or   : BExp → BExp → BExp
+namespace Exp
+open UOp BOp Const
 
--- Commands
-inductive Com
-| skip  : Com
-| set   : String → AExp → Com
-| seq   : Com → Com → Com
-| cond  : BExp → Com → Com → Com
-| while : BExp → Com → Com
+private def ci := λ n => const $ int n
+private def cb := λ b => const $ bool b
+
+def ex1 : Exp := (ci 42)
+def ex2 : Exp := (cb true)
+def ex3 : Exp := (uop inc (ci 41))
+def ex4 : Exp := (uop dec (const (int 43)))
+def ex5 : Exp := (uop neg (bop sub (ci 0) (ci 42)))
+def ex6 : Exp := (uop zero? (ci 0))
+def ex7 : Exp := (bop add (ci 41) (ci 1))
+def ex8 : Exp := (bop sub (ci 43) (ci 1))
+def ex9 : Exp := (bop mul (ci 21) (ci 2))
+def ex10 : Exp := (uop not (uop zero? (ci 1)))
+def ex11 : Exp := (cond (uop not (uop zero? (ci 42))) (ci 42) (ci 0))
+def ex12 : Exp := (cond (uop not (uop zero? (ci 0))) (ci 0) (ci 42))
+def ex13 : Exp := (letvar "x" (cb true)
+                    (cond (var "x") (ci 42) (ci 0)))
+def ex14 : Exp := (letvar "x" (uop inc (ci 41))
+                    (cond (cb true) (var "x") (ci 0)))
+def ex15 : Exp := (letvar "x" (uop inc (ci 39))
+                    (letvar "x" (uop inc (var "x"))
+                      (uop inc (var "x"))))
+
+end Exp
+
+def Env : Type := Var → Option Const
+
+namespace Env
+
+def empty : Env := λ _ => none
+def extend (ρ : Env) (x : Var) (c:Const) : Env :=
+  λ y => if x == y then some c else (ρ y)
+
+end Env
 
 -- -- -- -- -- -- -- -- -- -- -- -- -- -- -- -- --
--- Evaluation Functions
+-- Interpreter
 -- -- -- -- -- -- -- -- -- -- -- -- -- -- -- -- --
 
+namespace UOp
 
-def State : Type := String → Nat
+def interp : UOp → Const → Option Const
+| inc,   (Const.int n)  => some $ Const.int $ n + 1
+| dec,   (Const.int n)  => some $ Const.int $ n - 1
+| neg,   (Const.int n)  => some $ Const.int $ 0 - n
+| zero?, (Const.int n)  => some $ Const.bool $ n == 0
+| not,   (Const.bool b) => some $ Const.bool $ ¬ b
+| _,_ => none
 
-def init_state : State := λ _ => 0
+end UOp
 
-namespace AUOp
-open Nat
+namespace BOp
 
-def eval : AUOp → Nat → Nat
-| inc, n => n + 1
-| dec, 0 => 0
-| dec, (succ n) => n
+def interp : BOp → Const → Const → Option Const
+| add, (Const.int x), (Const.int y)  => some $ Const.int $ x + y
+| sub, (Const.int x), (Const.int y)  => some $ Const.int $ x - y
+| mul, (Const.int x), (Const.int y)  => some $ Const.int $ x * y
+| _,_,_ => none
 
-end AUOp
+end BOp
 
-namespace ABOp
 
-def eval : ABOp → Nat → Nat → Nat
-| add, x, y => x + y
-| sub, x, y => x - y
-| mul, x, y => x * y
+namespace Exp
 
-end ABOp
-
-namespace AExp
-
-def eval : State → AExp → Nat
-| _, num n => n
+def interp : Env → Exp → Option Const
 | ρ, var x => ρ x
-| ρ, uop op e => op.eval (e.eval ρ)
-| ρ, bop op e₁ e₂ => op.eval (e₁.eval ρ) (e₂.eval ρ)
+| ρ, const c => c
+| ρ, uop op e => do
+  v ← interp ρ e;
+  UOp.interp op v
+| ρ, bop op e₁ e₂ => do
+  v₁ ← interp ρ e₁;
+  v₂ ← interp ρ e₂;
+  BOp.interp op v₁ v₂
+| ρ, cond e₁ e₂ e₃ =>
+  match interp ρ e₁ with
+  | some (Const.bool true) => interp ρ e₂
+  | some (Const.bool false) => interp ρ e₃
+  | _ => none
+| ρ, letvar x e₁ e₂ => do
+  v₁ ← interp ρ e₁;
+  let ρ' := Env.extend ρ x v₁;
+  interp ρ' e₂
 
-namespace Tests
-open AUOp ABOp
-#eval (num 42).eval init_state == 42
-#eval (var "x").eval init_state == 0
-#eval ((uop inc) (var "x")).eval init_state == 1
-#eval ((uop dec) (num 42)).eval init_state == 41
-#eval ((bop add) (num 42) ((uop inc) (num 1))).eval init_state == 44
-end Tests
-
-end AExp
-
-
-
-namespace BBOp
-
-def eval : BBOp → Nat → Nat  → Bool
-| eq, n₁, n₂ => n₁ == n₂
-| le, n₁, n₂ => n₁ <= n₂
-
-end BBOp
+end Exp
 
 
-namespace BExp
-open BBOp
+def TyEnv : Type := Var → Option Ty
 
-def eval : State → BExp → Bool
-| _, bool b => b
-| ρ, bop op e₁ e₂ => op.eval (e₁.eval ρ) (e₂.eval ρ)
-| ρ, not e₁ => ¬ e₁.eval ρ
-| ρ, and e₁ e₂ => e₁.eval ρ && e₂.eval ρ
-| ρ, or e₁ e₂ => e₁.eval ρ || e₂.eval ρ
+namespace TyEnv
 
-namespace Tests
-open AExp AUOp ABOp
-#eval (bool true).eval init_state == true
-#eval (bop eq (num 1) (num 1)).eval init_state == true
-#eval (bop le (num 1) (num 1)).eval init_state == true
-#eval (bop le (num 1) (num 2)).eval init_state == true
-#eval (bop le (num 2) (num 1)).eval init_state == false
-#eval (not (bool true)).eval init_state == false
-#eval (and (bool true) (bool false)).eval init_state == false
-#eval (or (bool false) (bool true)).eval init_state == true
-end Tests
+def empty : TyEnv := λ _ => none
+def extend (Γ : TyEnv) (x : Var) (t:Ty) : TyEnv :=
+  λ y => if x == y then some t else (Γ y)
 
-end BExp
-
--- Environment extension
-def ext (p : String × Nat) (ρ : State) : State :=
-λ y => if p.fst == y then p.snd else ρ y
-
--- Single-step reduction relation
-inductive Step : State → Com → State → Prop
-| skip (ρ:State) : 
-  Step ρ Com.skip ρ
-| set (ρ:State) (e:AExp) (n:Nat) (x:String) : 
-  e.eval ρ = n 
-  → Step ρ (Com.set x e) (ext (x,n) ρ)
-| seq (ρ₁ ρ₂ ρ₃:State) (c₁ c₂:Com) :
-  Step ρ₁ c₁ ρ₂
-  → Step ρ₂ c₂ ρ₃
-  → Step ρ₁ (Com.seq c₁ c₂) ρ₃
-| if_true (ρ₁ ρ₂:State) (e:BExp) (c₁ c₂:Com) :
-  e.eval ρ₁ = true
-  → Step ρ₁ c₁ ρ₂
-  → Step ρ₁ (Com.cond e c₁ c₂) ρ₂
-| if_false (ρ₁ ρ₂:State) (e:BExp) (c₁ c₂:Com) :
-  e.eval ρ₁ = false
-  → Step ρ₁ c₂ ρ₂
-  → Step ρ₁ (Com.cond e c₁ c₂) ρ₂
-| while_false (e:BExp) (ρ:State) (c:Com) :
-  e.eval ρ = false
-  → Step ρ (Com.while e c) ρ
+end TyEnv
 
 
+namespace Const
 
--- def eval : Nat → Com → State → State 
+def typeof : Const → Ty
+| int _ => Ty.int
+| bool _ => Ty.bool
 
---def aeval : AExp → Nat
---| num n => n
---| 
+end Const
 
+
+namespace UOp
+
+def typeof : UOp → (Ty × Ty)
+| inc   => (Ty.int, Ty.int)
+| dec   => (Ty.int, Ty.int)
+| neg   => (Ty.int, Ty.int)
+| zero? => (Ty.int, Ty.bool)
+| not   => (Ty.bool, Ty.bool)
+end UOp
+
+
+namespace BOp
+
+def typeof : BOp → (Ty × Ty × Ty)
+| add   => (Ty.int, Ty.int, Ty.int)
+| sub   => (Ty.int, Ty.int, Ty.int)
+| mul   => (Ty.int, Ty.int, Ty.int)
+
+end BOp
+
+
+inductive TypeOf : TyEnv → Exp → Ty → Prop
+| var (Γ:TyEnv) x t :
+  (Γ x) = (some t)
+  → TypeOf Γ (Exp.var x) t
+| const Γ c t :
+  Const.typeof c = t
+  → TypeOf Γ (Exp.const c) t
+| uop Γ op e t t' :
+  TypeOf Γ e t
+  → UOp.typeof op = (t, t')
+  → TypeOf Γ (Exp.uop op e) t'
+| bop Γ op e₁ e₂ t₁ t₂ t₃ :
+  TypeOf Γ e₁ t₁
+  → TypeOf Γ e₂ t₂
+  → BOp.typeof op = (t₁, t₂, t₃)
+  → TypeOf Γ (Exp.bop op e₁ e₂) t₃
+| cond Γ e₁ e₂ e₃ t :
+  TypeOf Γ e₁ Ty.bool
+  → TypeOf Γ e₂ t
+  → TypeOf Γ e₃ t
+  → TypeOf Γ (Exp.cond e₁ e₂ e₃) t
+| letvar Γ x e₁ e₂ t₁ t₂ :
+  TypeOf Γ e₁ t₁
+  → TypeOf (TyEnv.extend Γ x t₁) e₂ t₂
+  → TypeOf Γ (Exp.letvar x e₁ e₂) t₂
+
+-- In the given expression, substitute
+-- the constant for the variable.
+def subst : Exp → Const → Var → Exp
+| Exp.var y, c, x => 
+  if x == y then (Exp.const c) else Exp.var y
+| Exp.const c, _, _ => 
+  Exp.const c
+| Exp.uop op e, c, x => 
+  Exp.uop op (subst e c x)
+| Exp.bop op e₁ e₂, c, x => 
+  Exp.bop op (subst e₁ c x) (subst e₂ c x)
+| Exp.cond e₁ e₂ e₃, c, x => 
+  Exp.cond (subst e₁ c x) (subst e₂ c x) (subst e₃ c x)
+| Exp.letvar y e₁ e₂, c, x => 
+  let e₁' := (subst e₁ c x);
+  if x == y then
+    Exp.letvar y e₁' e₂
+  else
+    Exp.letvar y e₁' (subst e₂ c x)
+
+-- A single reduction step.
+inductive Step : Exp → Exp → Prop 
+| uop_red op c₁ c₂ :
+  UOp.interp op c₁ = some c₂
+  → Step (Exp.uop op (Exp.const c₁)) (Exp.const c₂)
+| bop_red op c₁ c₂ c₃ :
+  BOp.interp op c₁ c₂ = some c₃
+  → Step (Exp.bop op (Exp.const c₁) (Exp.const c₂)) (Exp.const c₃)
+| cond_congr e₁ e₁' e₂ e₃ :
+  Step e₁ e₁'
+  → Step (Exp.cond e₁ e₂ e₃) (Exp.cond e₁' e₂ e₃)
+| cond_red e₁ e₂ :
+  Step (Exp.cond (Exp.const true) e₁ e₂) e₁
+| letvar_congr x e₁ e₁' e₂ :
+  Step e₁ e₁'
+  → Step (Exp.letvar x e₁ e₂) (Exp.letvar x e₁' e₂)
+| letvar_red x c e :
+  Step (Exp.letvar x (Exp.const c) e) (subst e c x)
+
+
+-- | Zero or more steps of reduction.
+inductive Steps : Exp → Exp → Prop
+| nil e : 
+  Steps e e
+| cons e₁ e₂ e₃ : 
+  Step e₁ e₂
+  → Steps e₂ e₃
+  → Steps e₁ e₃
+
+
+
+def env_sat (Γ:TyEnv) (ρ:Env) : Prop := forall x t, 
+   (Γ x) = some t 
+   → Exists (λ c => (ρ x) = some c ∧ Const.typeof c = t)
+
+
+
+-- -- -- -- -- -- -- -- -- -- -- -- -- -- -- -- --
+-- -- -- -- -- -- -- -- -- -- -- -- -- -- -- -- --
+-- -- -- -- -- -- -- -- -- -- -- -- -- -- -- -- --
+-- -- -- -- -- -- -- -- -- -- -- -- -- -- -- -- --
+-- -- -- -- -- -- -- -- -- -- -- -- -- -- -- -- --
+-- -- -- -- -- -- -- -- -- -- -- -- -- -- -- -- --
+-- Theorems (N.B., seems like tactics have to
+-- come after `new_frontend`... need to look
+-- more into what it entails.)
+-- -- -- -- -- -- -- -- -- -- -- -- -- -- -- -- --
+-- -- -- -- -- -- -- -- -- -- -- -- -- -- -- -- --
+-- -- -- -- -- -- -- -- -- -- -- -- -- -- -- -- --
+-- -- -- -- -- -- -- -- -- -- -- -- -- -- -- -- --
+-- -- -- -- -- -- -- -- -- -- -- -- -- -- -- -- --
+-- -- -- -- -- -- -- -- -- -- -- -- -- -- -- -- --
+
+
+
+new_frontend
+
+macro try t:tactic : tactic => `($t <|> skip)
+
+syntax "repeat" tactic : tactic
+macro_rules
+| `(tactic| repeat $t) => `(tactic| try ($t; repeat $t))
+
+-- TODO there's got to be a way to just apply all
+-- the known constructors for a type, right?
+-- oooh, check out src/Init/Lean/Meta/Tactic
+macro constr_TypeOf : tactic => 
+`((apply TypeOf.var) <|>
+  (apply TypeOf.const) <|>
+  (apply TypeOf.uop) <|>
+  (apply TypeOf.bop) <|>
+  (apply TypeOf.cond) <|>
+  (apply TypeOf.letvar))
+
+macro typecheck : tactic =>
+ `(repeat (constr_TypeOf <|> (exact rfl)))
+  
+
+
+open Exp
+
+-- -- -- -- -- -- -- -- -- -- -- -- -- -- -- -- --
+-- Example evaluation tests
+-- -- -- -- -- -- -- -- -- -- -- -- -- -- -- -- --
+
+def test_eval : Exp → Option Const := interp Env.empty
+
+private theorem test_ex1 : 
+ test_eval ex1 = some (Const.int 42) := 
+Eq.refl (some (Const.int 42))
+
+private theorem test_ex2 :
+ test_eval ex2 = some (Const.bool true) :=
+Eq.refl (some (Const.bool true))
+
+private theorem test_ex3 :
+ test_eval ex3 = some (Const.int 42) :=
+Eq.refl (some (Const.int 42))
+
+private theorem test_ex4 :
+ test_eval ex4 = some (Const.int 42) :=
+Eq.refl (some (Const.int 42))
+
+private theorem test_ex5 :
+ test_eval ex5 = some (Const.int 42) :=
+Eq.refl (some (Const.int 42))
+
+private theorem test_ex6 :
+ test_eval ex6 = some (Const.bool true) :=
+Eq.refl (some (Const.bool true))
+
+private theorem test_ex7 :
+ test_eval ex7 = some (Const.int 42) :=
+Eq.refl (some (Const.int 42))
+
+private theorem test_ex8 :
+ test_eval ex8 = some (Const.int 42) :=
+Eq.refl (some (Const.int 42))
+
+private theorem test_ex8 :
+ test_eval ex8 = some (Const.int 42) :=
+Eq.refl (some (Const.int 42))
+
+private theorem test_ex9 :
+ test_eval ex9 = some (Const.int 42) :=
+Eq.refl (some (Const.int 42))
+
+private theorem test_ex10 :
+ test_eval ex10 = some (Const.bool true) :=
+Eq.refl (some (Const.bool true))
+
+private theorem test_ex11 :
+ test_eval ex11 = some (Const.int 42) :=
+Eq.refl (some (Const.int 42))
+
+private theorem test_ex12 :
+ test_eval ex12 = some (Const.int 42) :=
+Eq.refl (some (Const.int 42))
+
+private theorem test_ex13 :
+ test_eval ex13 = some (Const.int 42) :=
+Eq.refl (some (Const.int 42))
+
+private theorem test_ex14 :
+ test_eval ex14 = some (Const.int 42) :=
+Eq.refl (some (Const.int 42))
+
+theorem test_ex15 : 
+ test_eval ex15 = some (Const.int 42) :=
+begin
+  exact rfl
+end
+
+-- -- -- -- -- -- -- -- -- -- -- -- -- -- -- -- --
+-- Example type checking tests
+-- -- -- -- -- -- -- -- -- -- -- -- -- -- -- -- --
+
+namespace Exp
+open UOp BOp Const
+
+
+theorem test_ex1 : 
+ TypeOf TyEnv.empty ex1 Ty.int :=
+begin
+  typecheck
+end
+
+theorem test_ex2 : 
+ TypeOf TyEnv.empty ex2 Ty.bool :=
+begin
+  typecheck
+end
+
+theorem test_ex3 : 
+ TypeOf TyEnv.empty ex3 Ty.int :=
+begin
+  typecheck
+end
+
+theorem test_ex4 : 
+ TypeOf TyEnv.empty ex4 Ty.int :=
+begin
+  typecheck
+end
+
+theorem test_ex5 : 
+ TypeOf TyEnv.empty ex5 Ty.int :=
+begin
+  typecheck
+end
+
+theorem test_ex6 : 
+ TypeOf TyEnv.empty ex6 Ty.bool :=
+begin
+  typecheck
+end
+
+theorem test_ex7 : 
+ TypeOf TyEnv.empty ex7 Ty.int :=
+begin
+  typecheck
+end
+
+theorem test_ex8 : 
+ TypeOf TyEnv.empty ex8 Ty.int :=
+begin
+  typecheck
+end
+
+theorem test_ex9 : 
+ TypeOf TyEnv.empty ex9 Ty.int :=
+begin
+  typecheck
+end
+
+theorem test_ex10 : 
+ TypeOf TyEnv.empty ex10 Ty.bool :=
+begin
+  typecheck
+end
+
+theorem test_ex11 : 
+ TypeOf TyEnv.empty ex11 Ty.int :=
+begin
+  typecheck
+end
+
+theorem test_ex12 : 
+ TypeOf TyEnv.empty ex12 Ty.int :=
+begin
+  typecheck
+end
+
+theorem test_ex13 : 
+ TypeOf TyEnv.empty ex13 Ty.int :=
+begin
+  typecheck
+end
+
+theorem test_ex14 : 
+ TypeOf TyEnv.empty ex14 Ty.int :=
+begin
+  typecheck
+end
+
+theorem test_ex15 : 
+ TypeOf TyEnv.empty ex15 Ty.int :=
+begin
+  typecheck
+end
+
+
+end Exp
+
+
+-- -- -- -- -- -- -- -- -- -- -- -- -- -- -- -- --
+-- Type safety theorems
+-- -- -- -- -- -- -- -- -- -- -- -- -- -- -- -- --
+
+namespace UOp
+open Const
+
+def interp_safe : forall op t₁ t₂ c,
+ typeof op = (t₁, t₂)
+ → Const.typeof c = t₁
+ → Exists (λ c' => interp op c = some c' ∧ Const.typeof c' = t₂) :=
+begin
+  intros op t₁ t₂ c Hop Hc;
+  cases op; cases c;
+  apply (Exists.intro (Const.int $ a + 1));
+  apply And.intro;
+  exact rfl;
+end
+
+end UOp
+
+
+-- UOp.interp is type safe
+-- BOp.interp is type safe
+-- BOp.interp is type safe
 
